feat: Add Coq elaborator implementation and partial well-scopedness lemma
Implementation of #8 is currently incomplete.

lib/elaborator.v
@@ -1,5 +1,14 @@
 Require Export String.
 Require Export List.
+Require Export Coq.Structures.OrderedTypeEx.
+Require Export MSets MSetInterface MSetFacts MSetProperties.
+Require Export Arith.
+
+Open Scope string_scope.
+
+
+Module StrSet := Make String_as_OT.
+Module StrSProp := MSetProperties.Properties StrSet.
 
 
 Inductive cst_term : Type :=
@@ -25,25 +34,9 @@ Inductive ast_term : Type :=
 Fixpoint lookup (s : string) (ctx : list string) (index : nat) : (option nat) :=
  match ctx with
   | nil => None
-  | c::cs => if eqb c s then (Some index) else lookup s cs (index+1) 
+  | c::cs => if String.eqb c s then (Some index) else lookup s cs (index+1) 
  end
 .
-
-
-
-Definition ret {A : Type} (x : A) := Some x.
-
-Definition bind {A B : Type} (a : option A) (f : A -> option B) : option B :=
-  match a with
-    | Some x => f x
-    | None => None
-  end.
-
-Notation "A >>= F" := (bind A F) (at level 42, left associativity).
-
-Search (  option ?A -> (?A-> option ?B) -> option ?B).
-
-Definition compose {A B C : Type} (f : A -> B) (g : B -> C) : A -> C := fun x => g (f x).
 
 
 Fixpoint elaborate (cst : cst_term) (ctx : list string) : (option ast_term) :=
@@ -51,12 +44,274 @@ Fixpoint elaborate (cst : cst_term) (ctx : list string) : (option ast_term) :=
  | cType n => Some (aType n)
  | cNat => Some aNat
  | cZero => Some aZero
- | cSucc c => (elaborate c ctx) >>= (compose aSucc ret)
- | cVar s =>  (lookup s ctx 0) >>= (compose aVar ret)
- | cFun s c => (elaborate c (s::ctx)) >>= (compose aFun ret)
- | cApp c1 c2 => (elaborate c1 ctx) >>= (fun c1 => (elaborate c2 ctx) >>= (compose (aApp c1) ret))
+ | cSucc c => match elaborate c ctx with
+              | Some a => Some (aSucc a)
+              | None => None
+              end
+ | cVar s =>  match lookup s ctx 0 with
+              | Some n => Some (aVar n)
+              | None => None
+              end
+ | cFun s c => match (elaborate c (s::ctx)) with
+              | Some a => Some (aFun a)
+              | None => None
+              end 
+ | cApp c1 c2 => match elaborate c1 ctx, elaborate c2 ctx with
+              | None, _ => None
+              | _, None => None
+              | Some a1, Some a2 => Some (aApp a1 a2)
+              end 
  end
 .
+
+Fixpoint cst_variables (cst : cst_term) : StrSet.t :=
+ match cst with
+  | cType n => StrSet.empty
+  | cNat => StrSet.empty
+  | cZero => StrSet.empty
+  | cSucc c => cst_variables c
+  | cVar s => StrSet.singleton s
+  | cFun s c => StrSet.remove s (cst_variables c)
+  |cApp c1 c2 => StrSet.union (cst_variables c1) (cst_variables c2)
+ end
+.
+
+Fixpoint max_index (ast : ast_term) : option nat :=
+  match ast with
+    | aType n => None
+    | aNat => None
+    | aZero => None
+    | aSucc a => max_index a
+    | aVar n => Some n
+    | aFun a => max_index a
+    | aApp a1 a2 => match (max_index a1), (max_index a2) with
+                    | Some n1, None => Some n1
+                    | None, Some n2 => Some n2
+                    | Some n1, Some n2 => Some (max n1 n2)
+                    | None, None => None
+                    end
+  end
+.
+
+Lemma lookup_immediate (s: string) (ctx: list string) (k : nat) : lookup s (s::ctx) k = Some k.
+Proof.
+  simpl.
+  assert (se := String.eqb_eq s s).
+  assert (b : s =? s = true).
+  assert (ssym : s = s) by reflexivity.
+  destruct se.
+  exact (H0 ssym).
+  rewrite b.
+  reflexivity.
+Qed.
+
+Lemma lookup_next (s c: string) (ctx: list string) (neq : s <> c) (n: nat) : (lookup s ctx (n+1) = lookup s (c::ctx) (n)).
+Proof.
+  simpl.
+  assert (c =? s = false).
+  rewrite eqb_sym.
+  apply String.eqb_neq.
+  exact neq.
+  rewrite H.
+  reflexivity.
+Qed.
+
+Lemma additive_identity_unique (m n : nat) (e : m = m + n): (n = 0).
+Proof.
+  induction m.
+  simpl in e.
+  symmetry.
+  exact e.
+  inversion e.
+  exact (IHm H0).
+Qed.
+Lemma lookup_lemma (s : string) (ctx: list string) (n m: nat) (p : lookup s ctx n = Some (n+m)) : lookup s ctx (n+1) = Some (n+m+1).
+(*Proof.
+  induction ctx as [| c ctx' IHctx].
+  simpl.
+  discriminate.
+
+  assert (str_dec := String.string_dec s c).
+  destruct str_dec.
+  simpl.
+
+  assert (eqcs : c =? s = true).
+  apply (String.eqb_eq c s).
+  symmetry.
+  exact e.
+
+  rewrite eqcs.
+  
+  
+  assert (P := lookup_immediate c ctx').
+  rewrite -> e in p.
+  rewrite -> (P n) in p.
+  assert(m=0). { inversion p. apply (additive_identity_unique n m H0). }
+  rewrite H.
+  auto.
+
+  rewrite <- ((lookup_next s c ctx' n0 n)) in p.
+  simpl.
+
+  assert (c =? s = false).
+    { rewrite eqb_sym. apply String.eqb_neq. exact n0. }
+
+  rewrite H.
+
+  assert (Q := lookup_next s c ctx' n0 n).
+  *)
+Admitted.
+
+Lemma lookup_known (s : string) (ctx : list string) (p : List.In s ctx) : exists n : nat, (lookup s ctx 0 = Some n).
+Proof.
+  
+  
+  induction ctx as [| c ctx' IHctx].
+  simpl.
+  contradiction.
+
+  
+  
+  assert (str_dec := String.string_dec s c).
+  destruct str_dec.
+  
+  simpl.
+  exists 0.
+  assert (eqcs : c =? s = true).
+  apply (String.eqb_eq c s).
+  symmetry.
+  exact e.
+
+  rewrite eqcs.
+  simpl.
+  reflexivity.
+  
+  assert (In s ctx').
+  assert (H := List.in_inv p).
+  destruct H.
+  destruct n.
+  symmetry.
+  exact H.
+  exact H.
+
+  assert (I := In_nth ctx' s "" H).
+  destruct(I).
+  destruct(H0).
+  destruct (IHctx H).
+
+  simpl.
+  assert (Q : s =? c = false).
+  apply eqb_neq.
+  exact n.
+  rewrite eqb_sym.
+  rewrite Q.
+  exists(x0 + 1).
+  
+  assert (L:=(lookup_lemma s ctx' 0 x0) H3).
+  simpl in L.
+  exact L.
+Qed.
+
+
+(* If all free variables are in a context, then elaboration suceeds with that context*)
+Lemma well_scoped (cst : cst_term) (ctx : list string) 
+(x : StrSet.Subset (cst_variables cst) (StrSProp.of_list ctx)) :
+exists a : ast_term, and (elaborate cst ctx = Some a) 
+               (or ((max_index a) = None) (exists n : nat, and (max_index a = Some n) (n = StrSet.cardinal (cst_variables cst)))).
+Proof.
+  induction cst.
+
+  exists (aType level).
+  split.
+  reflexivity.
+  left.
+  reflexivity.
+  
+
+  exists (aNat).
+  split.
+  reflexivity.
+  left.
+  reflexivity.
+  
+  assert (StrSet.In s (cst_variables (cVar s))). {
+    simpl.
+    apply (StrSet.singleton_spec).
+    reflexivity. }
+  assert (In s ctx). {
+    assert (Q:=StrSProp.of_list_1 ctx s).
+    assert (InA eq s ctx -> In s ctx).
+    intro.
+    rewrite (InA_alt eq s ctx) in H0.
+    destruct H0.
+    destruct H0.
+    rewrite <- H0 in H1.
+    exact H1.
+    rewrite <- Q in H0.
+    apply H0.
+    auto. }
+
+
+  destruct (lookup_known s ctx H0).
+  exists (aVar x0).
+  simpl.
+  rewrite H1.
+  split.
+  reflexivity.
+  right.
+  exists 1.
+  split.
+
+  2: auto.
+
+  
+  
+  
+  (*exists aZero.
+  auto.
+  auto.
+  assert (I := IHcst x).
+  destruct I.
+  exists (aSucc x0).
+  simpl.
+  rewrite H.
+  reflexivity.
+
+  assert(StrSet.Subset (cst_variables (cst)) (StrSProp.of_list ctx)) by admit.
+
+  assert (I := IHcst H).
+  destruct I.
+  exists (aFun x0).
+  simpl.
+ 
+  
+  assert (elaborate cst ctx = elaborate cst (s :: ctx)) by admit.
+  
+  rewrite <- H1.
+  rewrite H0.
+  reflexivity.
+  
+ 
+  assert (StrSet.Subset (cst_variables cst1) (cst_variables (cApp cst1 cst2))).
+  simpl.
+  apply StrSProp.union_subset_1.
+  assert (S1 : StrSet.Subset (cst_variables cst1) (StrSProp.of_list ctx)).
+  apply (StrSProp.subset_trans H x).
+  destruct (IHcst1 S1).
+
+  assert (StrSet.Subset (cst_variables cst2) (cst_variables (cApp cst1 cst2))).
+  simpl.
+  apply StrSProp.union_subset_2.
+  assert (S2 : StrSet.Subset (cst_variables cst2) (StrSProp.of_list ctx)).
+  apply (StrSProp.subset_trans H1 x).
+  destruct (IHcst2 S2).
+  
+  exists(aApp x0 x1).
+  simpl.
+  rewrite H2.
+  rewrite H0.
+  reflexivity.*)
+Qed.
 
 Check elaborate cNat nil : option ast_term.
 Fail Check elaborate (cSucc aNat) : option ast_term.
